# SPDX-FileCopyrightText: Â© 2023 Dominik George <nik@naturalnet.de>
#
# SPDX-License-Identifier: LGPL-3.0-or-later OR CC-BY-SA-4.0+

@prefix : <https://docs.vocata.one/information-schema#> .
@prefix owl: <http://www.w3.org/2002/07/owl#> .
@prefix rdf: <http://www.w3.org/1999/02/22-rdf-syntax-ns#> .
@prefix xml: <http://www.w3.org/XML/1998/namespace> .
@prefix xsd: <http://www.w3.org/2001/XMLSchema#> .
@prefix rdfs: <http://www.w3.org/2000/01/rdf-schema#> .
@base <https://docs.vocata.one/information-schema> .

<https://docs.vocata.one/information-schema> rdf:type owl:Ontology ;
                                              owl:imports <http://www.w3.org/ns/activitystreams#> ;
                                              rdfs:comment """Internal information schema for Vocata.

Used to track state that is local to the Vocata graph and server. Statements using properties in this schema MUST NOT be federated over ActivityPub.""" ;
                                              rdfs:label "Vocata Information Schema" .

#################################################################
#    Data properties
#################################################################

###  https://docs.vocata.one/information-schema#hashedPassword
:hashedPassword rdf:type owl:DatatypeProperty ;
                rdfs:subPropertyOf owl:topDataProperty ;
                rdf:type owl:FunctionalProperty ;
                rdfs:domain <http://www.w3.org/ns/activitystreams#Object> ;
                rdfs:range xsd:string ;
                rdfs:comment """Hashed password this actor can use to login to Vocata.

MUST be a hash in PBKDF2-SHA512 format.""" ;
                rdfs:label "Hashed password (PBKDF2-SHA512)" .


###  https://docs.vocata.one/information-schema#isLocal
:isLocal rdf:type owl:DatatypeProperty ;
         rdfs:subPropertyOf owl:topDataProperty ;
         rdf:type owl:FunctionalProperty ;
         rdfs:domain <http://www.w3.org/ns/activitystreams#Service> ;
         rdfs:range xsd:boolean ;
         rdfs:comment """Determines whether this Service denotes a URI prefix owned by this Vocata server.

The object IR MUST NOT have a path component, and it SHOULD be a Service actor.""" ;
         rdfs:label "Is local prefix" .

###  https://docs.vocata.one/information-schema#role
:hasServerRole rdf:type owl:DatatypeProperty ;
         rdfs:subPropertyOf owl:topDataProperty ;
         rdf:type owl:FunctionalProperty ;
         rdfs:domain <http://www.w3.org/ns/activitystreams#Actor> ;
         rdfs:range xsd:string ;
         rdfs:comment """Determines the role this Actor has on this Vocata server.

The object IR MUST NOT have a path component, and it SHOULD be a Service actor.""" ;
         rdfs:label "Is local prefix" .

###  https://docs.vocata.one/information-schema#processResult
:processResult rdf:type owl:DatatypeProperty ;
               rdfs:subPropertyOf owl:topDataProperty ;
               rdfs:domain <http://www.w3.org/ns/activitystreams#Activity> ;
               rdfs:range xsd:string ;
               rdfs:comment "Human-readable status from processing" ;
               rdfs:label "Processing result" .


###  https://docs.vocata.one/information-schema#processed
:processed rdf:type owl:DatatypeProperty ;
           rdfs:subPropertyOf owl:topDataProperty ;
           rdf:type owl:FunctionalProperty ;
           rdfs:domain <http://www.w3.org/ns/activitystreams#Activity> ;
           rdfs:range xsd:boolean ;
           rdfs:comment "Whether the activity was processed and its side effects carried out" ;
           rdfs:label "Processed" .


###  https://docs.vocata.one/information-schema#processedAt
:processedAt rdf:type owl:DatatypeProperty ;
             rdfs:subPropertyOf owl:topDataProperty ;
             rdf:type owl:FunctionalProperty ;
             rdfs:domain <http://www.w3.org/ns/activitystreams#Activity> ;
             rdfs:range xsd:dateTime ;
             rdfs:comment "Date and time the activity was processed and its side effects carried out (if successful)" ;
             rdfs:label "Processed at" .


###  https://docs.vocata.one/information-schema#receivedAt
:receivedAt rdf:type owl:DatatypeProperty ;
            rdfs:subPropertyOf owl:topDataProperty ;
            rdf:type owl:FunctionalProperty ;
            rdfs:domain <http://www.w3.org/ns/activitystreams#Object> ;
            rdfs:range xsd:dateTime ;
            rdfs:comment "Date and time the object was received through a POST to a box" ;
            rdfs:label "Received at" .


###  Generated by the OWL API (version 4.5.25.2023-02-15T19:15:49Z) https://github.com/owlcs/owlapi
